
Please see file ``sumsq.v'' to follow along with this example. 

~\\
In this example, we define the function \TT{sumsq}, or the sum of squares 
(i.e., \TT{$\Sigma_{i=0}^n\ (i * i)$}). 



\begin{code}
\Load Arith.
\\ \\ 
\Fixpoint \nm{sumsq} (n: nat) : nat := 		\\ \-\ \quad
	\match n \with						\\ \-\ \qquad
	$\mid$ O $=>$ 0					\\ \-\ \qquad
	$\mid$ S p $=>$ (n * n) + (sumsq p)		\\ \-\ \quad
	\End.
\end{code}

\noindent
We then want to prove that \TT{6 * sumsq n = n * (n + 1) * (2n + 1)} 
(or \TT{$sumsq\ n = \frac{n * (n + 1) * (2n + 1)}{6}$}). 





